feat(library/hott): add adjointification and closure properties for equivalences
Port features from the Coq Hott library

library/hott/equiv.lean
@@ -3,7 +3,7 @@
 -- Author: Jeremy Avigad
 -- Ported from Coq HoTT
 import .path
-open path
+open path function
 
 -- Equivalences
 -- ------------
@@ -15,27 +15,32 @@ definition Sect {A B : Type} (s : A → B) (r : B → A) := Πx : A, r (s x) ≈
 
 -- Structure IsEquiv
 
-inductive IsEquiv {A B : Type} (f : A → B) :=
+inductive IsEquiv [class] {A B : Type} (f : A → B) :=
 IsEquiv_mk : Π
-  (equiv_inv : B → A)
-  (eisretr : Sect equiv_inv f)
-  (eissect : Sect f equiv_inv)
-  (eisadj : Πx, eisretr (f x) ≈ ap f (eissect x)),
+  (inv : B → A)
+  (retr : Sect inv f)
+  (sect : Sect f inv)
+  (adj : Πx, retr (f x) ≈ ap f (sect x)),
 IsEquiv f
 
-definition equiv_inv {A B : Type} {f : A → B} (H : IsEquiv f) : B → A :=
-IsEquiv.rec (λequiv_inv eisretr eissect eisadj, equiv_inv) H
 
--- TODO: note: does not type check without giving the type
-definition eisretr {A B : Type} {f : A → B} (H : IsEquiv f) : Sect (equiv_inv H) f :=
-IsEquiv.rec (λequiv_inv eisretr eissect eisadj, eisretr) H
+namespace IsEquiv
 
-definition eissect {A B : Type} {f : A → B} (H : IsEquiv f) : Sect f (equiv_inv H) :=
-IsEquiv.rec (λequiv_inv eisretr eissect eisadj, eissect) H
+  definition inv {A B : Type} {f : A → B} (H : IsEquiv f) : B → A :=
+    IsEquiv.rec (λinv retr sect adj, inv) H
 
-definition eisadj {A B : Type} {f : A → B} (H : IsEquiv f) :
-  Πx, eisretr H (f x) ≈ ap f (eissect H x) :=
-IsEquiv.rec (λequiv_inv eisretr eissect eisadj, eisadj) H
+  -- TODO: note: does not type check without giving the type
+  definition retr {A B : Type} {f : A → B} (H : IsEquiv f) : Sect (inv H) f :=
+    IsEquiv.rec (λinv retr sect adj, retr) H
+
+  definition sect {A B : Type} {f : A → B} (H : IsEquiv f) : Sect f (inv H) :=
+    IsEquiv.rec (λinv retr sect adj, sect) H
+
+  definition adj {A B : Type} {f : A → B} (H : IsEquiv f) :
+	     Πx, retr H (f x) ≈ ap f (sect H x) :=
+    IsEquiv.rec (λinv retr sect adj, adj) H
+
+end IsEquiv
 
 -- Structure Equiv
 
@@ -45,12 +50,140 @@ Equiv_mk : Π
   (equiv_isequiv : IsEquiv equiv_fun),
 Equiv A B
 
-definition equiv_fun [coercion] {A B : Type} (e : Equiv A B) : A → B :=
-Equiv.rec (λequiv_fun equiv_isequiv, equiv_fun) e
+namespace Equiv
 
-definition equiv_isequiv [coercion] {A B : Type} (e : Equiv A B) : IsEquiv (equiv_fun e) :=
-Equiv.rec (λequiv_fun equiv_isequiv, equiv_isequiv) e
+  definition equiv_fun [coercion] {A B : Type} (e : Equiv A B) : A → B :=
+    Equiv.rec (λequiv_fun equiv_isequiv, equiv_fun) e
 
--- TODO: better symbol
-infix `<~>`:25 := Equiv
-notation H ⁻¹ := equiv_inv H
+  definition equiv_isequiv [coercion] {A B : Type} (e : Equiv A B) : IsEquiv (equiv_fun e) :=
+    Equiv.rec (λequiv_fun equiv_isequiv, equiv_isequiv) e
+
+  infix `≃`:25 := Equiv
+  notation e `⁻¹` := IsEquiv.inv e
+
+end Equiv
+
+  -- Some instances and closure properties of equivalences
+
+namespace IsEquiv
+  variables {A B C : Type} {f : A → B} {g : B → C} {f' : A → B}
+
+  -- The identity function is an equivalence.
+
+  definition idIsEquiv [instance] : (@IsEquiv A A id) := IsEquiv_mk id (λa, idp) (λa, idp) (λa, idp)
+
+  -- The composition of two equivalences is, again, an equivalence.
+
+  definition comp_closed [instance] (Hf : IsEquiv f) (Hg : IsEquiv g) : (IsEquiv (g ∘ f)) :=
+    IsEquiv_mk ((inv Hf) ∘ (inv Hg))
+	       (λc, ap g (retr Hf ((inv Hg) c)) @ retr Hg c)
+	       (λa, ap (inv Hf) (sect Hg (f a)) @ sect Hf a)
+	       (λa, (whiskerL _ (adj Hg (f a))) @
+		    (ap_pp g _ _)^ @
+		    ap02 g (concat_A1p (retr Hf) (sect Hg (f a))^ @
+			    (ap_compose (inv Hf) f _ @@ adj Hf a) @
+			    (ap_pp f _ _)^
+			   ) @
+		    (ap_compose f g _)^
+	       )
+
+  -- Any function equal to an equivalence is an equivlance as well.
+  definition path_closed (Hf : IsEquiv f) (Heq : f ≈ f') : (IsEquiv f') :=
+     path.induction_on Heq Hf
+
+  -- Any function pointwise equal to an equivalence is an equivalence as well.
+  definition homotopic (Hf : IsEquiv f) (Heq : f ∼ f') : (IsEquiv f') :=
+    let sect' := (λ b, (Heq (inv Hf b))^ @ retr Hf b) in
+    let retr' := (λ a, (ap (inv Hf) (Heq a))^ @ sect Hf a) in
+    let adj' := (λ (a : A),
+      let ff'a := Heq a in
+      let invf := inv Hf in
+      let secta := sect Hf a in
+      let retrfa := retr Hf (f a) in
+      let retrf'a := retr Hf (f' a) in
+      have eq1 : ap f secta @ ff'a ≈ ap f (ap invf ff'a) @ retr Hf (f' a),
+        from calc ap f secta @ ff'a
+              ≈ retrfa @ ff'a : (ap _ (adj Hf _ ))^
+          ... ≈ ap (f ∘ invf) ff'a @ retrf'a : !concat_A1p^
+          ... ≈ ap f (ap invf ff'a) @ retr Hf (f' a) : {ap_compose invf f ff'a},
+      have eq2 : retrf'a ≈ Heq (invf (f' a)) @ ((ap f' (ap invf ff'a))^ @ ap f' secta),
+        from calc retrf'a
+              ≈ (ap f (ap invf ff'a))^ @ (ap f secta @ ff'a) : moveL_Vp _ _ _ (eq1^)
+          ... ≈ ap f (ap invf ff'a)^ @ (ap f secta @ Heq a) : {ap_V invf ff'a}
+          ... ≈ ap f (ap invf ff'a)^ @ (Heq (invf (f a)) @ ap f' secta) : {!concat_Ap}
+          ... ≈ ap f (ap invf ff'a)^ @ Heq (invf (f a)) @ ap f' secta : {!concat_pp_p^}
+          ... ≈ ap f ((ap invf ff'a)^) @ Heq (invf (f a)) @ ap f' secta : {!ap_V^}
+          ... ≈ Heq (invf (f' a)) @ ap f' ((ap invf ff'a)^) @ ap f' secta : {!concat_Ap}
+          ... ≈ Heq (invf (f' a)) @ (ap f' (ap invf ff'a))^ @ ap f' secta : {!ap_V}
+          ... ≈ Heq (invf (f' a)) @ ((ap f' (ap invf ff'a))^ @ ap f' secta) : !concat_pp_p,
+      have eq3 : (Heq (invf (f' a)))^ @ retr Hf (f' a) ≈ ap f' ((ap invf ff'a)^ @ secta),
+        from calc (Heq (invf (f' a)))^ @ retr Hf (f' a)
+              ≈ (ap f' (ap invf ff'a))^ @ ap f' secta : moveR_Vp _ _ _ eq2
+          ... ≈ (ap f' ((ap invf ff'a)^)) @ ap f' secta : {!ap_V^}
+          ... ≈ ap f' ((ap invf ff'a)^ @ secta) : !ap_pp^,
+    eq3) in
+  IsEquiv_mk (inv Hf) sect' retr' adj'
+               
+  --TODO: Maybe wait until rewrite rules are available.
+  definition inv_closed (Hf : IsEquiv f) : (IsEquiv (inv Hf)) :=
+    IsEquiv_mk sorry sorry sorry sorry
+
+  definition cancel_R (Hf : IsEquiv f) (Hgf : IsEquiv (g ∘ f)) : (IsEquiv g) :=
+    homotopic (comp_closed (inv_closed Hf) Hgf) (λb, ap g (retr Hf b))
+
+  definition cancel_L (Hg : IsEquiv g) (Hgf : IsEquiv (g ∘ f)) : (IsEquiv f) :=
+    homotopic (comp_closed Hgf (inv_closed Hg)) (λa, sect Hg (f a))
+
+  definition transport (P : A → Type) {x y : A} (p : x ≈ y) : (IsEquiv (transport P p)) :=
+    IsEquiv_mk (transport P (p^)) (transport_pV P p) (transport_Vp P p) (transport_pVp P p)
+
+  --Rewrite rules
+  section
+  variables {Hf : IsEquiv f}
+  
+  definition moveR_M {x : A} {y : B} (p : x ≈ (inv Hf) y) : (f x ≈ y) :=
+    ap f p @ retr Hf y
+
+  definition moveL_M {x : A} {y : B} (p : (inv Hf) y ≈ x) : (y ≈ f x) :=
+    (moveR_M (p^))^
+
+  definition moveR_V {x : B} {y : A} (p : x ≈ f y) : (inv Hf) x ≈ y :=
+    ap (inv Hf) p @ sect Hf y
+
+  definition moveL_V {x : B} {y : A} (p : f y ≈ x) : y ≈ (inv Hf) x :=
+    (moveR_V (p^))^
+  
+  end
+
+end IsEquiv
+
+namespace Equiv
+
+  variables {A B C : Type} (eqf : A ≃ B)
+
+  theorem id : A ≃ A := Equiv_mk id IsEquiv.idIsEquiv
+
+  theorem compose (eqg: B ≃ C) : A ≃ C :=
+    Equiv_mk ((equiv_fun eqg) ∘ (equiv_fun eqf))
+	     (IsEquiv.comp_closed (equiv_isequiv eqf) (equiv_isequiv eqg))
+
+  check IsEquiv.path_closed
+
+  theorem path_closed (f' : A → B) (Heq : equiv_fun eqf ≈ f') : A ≃ B :=
+    Equiv_mk f' (IsEquiv.path_closed (equiv_isequiv eqf) Heq)
+
+  theorem inv_closed : B ≃ A :=
+    Equiv_mk (IsEquiv.inv (equiv_isequiv eqf)) (IsEquiv.inv_closed (equiv_isequiv eqf))
+
+  theorem cancel_L {f : A → B} {g : B → C} 
+                   (Hf : IsEquiv f) (Hgf : IsEquiv (g ∘ f)) : B ≃ C :=
+    Equiv_mk g (IsEquiv.cancel_R _ _)
+  
+  theorem cancel_R {f : A → B} {g : B → C}
+                   (Hg : IsEquiv g) (Hgf : IsEquiv (g ∘ f)) : A ≃ B :=
+    Equiv_mk f (!IsEquiv.cancel_L _ _)
+
+  theorem transport (P : A → Type) {x y : A} {p : x ≈ y} : (P x) ≃ (P y) :=
+    Equiv_mk (transport P p) (IsEquiv.transport P p)
+
+end Equiv
